Added Ictr with lca_as_prefix + distinct ops changes

Ictr.fst
@@ -7,6 +7,9 @@ open FStar.Ghost
 // e.g. for the increment only counter (icounter), concrete_st = nat
 type concrete_st = nat
 
+//initial state
+let init_st = 0
+
 // operation type
 // (the only operation is increment, so unit is fine)
 type op_t = unit
@@ -15,7 +18,7 @@ type op_t = unit
 let do (s:concrete_st) (_:log_entry) : concrete_st = s + 1
 
 let rec lem_foldl (s:concrete_st) (l:log)
-  : Lemma (ensures (seq_foldl do s l) = s + length l) 
+  : Lemma (ensures ((seq_foldl do s l) = s + length l))
           (decreases length l)
   = match length l with
     |0 -> ()
@@ -24,17 +27,6 @@ let rec lem_foldl (s:concrete_st) (l:log)
 //conflict resolution
 let resolve_conflict (x y:log_entry) : log =
   cons x (cons y empty)
-
-(*)let resolve_conflict_len (x y:log_entry)
-  : Lemma (Seq.length (resolve_conflict x y) = 2)
-  = ()
-
-let resolve_conflict_mem (x y:log_entry)
-  : Lemma (resolve_conflict_len x y;
-           let s = resolve_conflict x y in
-           (Seq.length s == 1 ==> is_x_or_y s x y) /\
-           (Seq.length s == 2 ==> is_x_and_y s x y))
-  = ()*)
 
 // concrete merge pre-condition
 let concrete_merge_pre lca a b : prop
@@ -45,47 +37,73 @@ let concrete_merge (lca:concrete_st) (cst1:concrete_st) (cst2:concrete_st{concre
   : concrete_st = cst1 + cst2 - lca
 
 let merge_prop (lca s1 s2:st)
-  : Lemma (requires v_of lca == init_of s1 /\
-                    init_of s1 == init_of s2) 
+  : Lemma (requires init_of lca == init_st /\
+                    init_of lca == init_of s1 /\
+                    init_of lca == init_of s2 /\ 
+                    is_prefix (ops_of lca) (ops_of s1) /\ 
+                    is_prefix (ops_of lca) (ops_of s2))
           (ensures concrete_merge_pre (v_of lca) (v_of s1) (v_of s2)) =
+  lem_foldl (init_of lca) (ops_of lca);
   lem_foldl (init_of s1) (ops_of s1);
   lem_foldl (init_of s2) (ops_of s2)
 
 let merge_inv_prop (lca s1 s2:st)
-  : Lemma (requires length (ops_of s1) > 0 /\ length (ops_of s2) > 0 /\
-                    v_of lca == init_of s1 /\
-                    init_of s1 == init_of s2)
+  : Lemma (requires length (ops_of s1) - length (ops_of lca) > 0 /\ 
+                    length (ops_of s2) - length (ops_of lca) > 0 /\
+                    init_of lca == init_st /\
+                    init_of lca == init_of s1 /\
+                    init_of lca == init_of s2 /\
+                    is_prefix (ops_of lca) (ops_of s1) /\ 
+                    is_prefix (ops_of lca) (ops_of s2))
           (ensures concrete_merge_pre (v_of lca) (v_of (inverse_st s1)) (v_of (inverse_st s2))) =
+  lem_foldl (init_of lca) (ops_of lca);
   lem_foldl (init_of s1) (ops_of (inverse_st s1));
   lem_foldl (init_of s2) (ops_of (inverse_st s2))
 
 let linearizable_s1_0 (lca s1 s2:st)
   : Lemma (requires 
-             v_of lca == init_of s1 /\
-             init_of s1 == init_of s2 /\
+             init_of lca == init_st /\
+             init_of lca == init_of s1 /\
+             init_of lca == init_of s2 /\ 
              concrete_merge_pre (v_of lca) (v_of s1) (v_of s2) /\
-             length (ops_of s1) = 0) 
-          (ensures 
-             concrete_merge (v_of lca) (v_of s1) (v_of s2) ==
-             seq_foldl do (v_of lca) (ops_of s2)) =
-  ()
+             is_prefix (ops_of lca) (ops_of s1) /\
+             is_prefix (ops_of lca) (ops_of s2) /\
+             Seq.length (diff (ops_of s1) (ops_of lca)) = 0) 
+           (ensures 
+              concrete_merge (v_of lca) (v_of s1) (v_of s2) == 
+              seq_foldl do (v_of lca) (diff (ops_of s2) (ops_of lca))) =
+  lem_foldl (v_of lca) (diff (ops_of s2) (ops_of lca));
+  lem_foldl (init_of lca) (ops_of lca);
+  lem_foldl (init_of s2) (ops_of s2)
 
 let linearizable_s2_0 (lca s1 s2:st)
   : Lemma (requires 
-             v_of lca == init_of s1 /\
-             init_of s1 == init_of s2 /\
+             init_of lca == init_st /\
+             init_of lca == init_of s1 /\
+             init_of lca == init_of s2 /\ 
              concrete_merge_pre (v_of lca) (v_of s1) (v_of s2) /\
-             length (ops_of s2) = 0) 
+             is_prefix (ops_of lca) (ops_of s1) /\
+             is_prefix (ops_of lca) (ops_of s2) /\
+             Seq.length (diff (ops_of s2) (ops_of lca)) = 0) 
           (ensures 
-             concrete_merge (v_of lca) (v_of s1) (v_of s2) ==
-             seq_foldl do (v_of lca) (ops_of s1)) =
-  ()
+             concrete_merge (v_of lca) (v_of s1) (v_of s2) == 
+             seq_foldl do (v_of lca) (diff (ops_of s1) (ops_of lca))) =
+  lem_foldl (v_of lca) (diff (ops_of s1) (ops_of lca));
+  lem_foldl (init_of s1) (ops_of s1);
+  lem_foldl (init_of lca) (ops_of lca)
 
+#set-options "--z3rlimit 50"
 let linearizable_s1s2_gt0 (lca s1 s2:st) (l':log)
   : Lemma (requires 
-             v_of lca == init_of s1 /\
-             init_of s1 == init_of s2 /\
-             length (ops_of s1) > 0 /\ length (ops_of s2) > 0 /\
+             init_of lca == init_st /\
+             init_of lca == init_of s1 /\
+             init_of lca == init_of s2 /\ 
+             is_prefix (ops_of lca) (ops_of s1) /\
+             is_prefix (ops_of lca) (ops_of s2) /\
+             Seq.length (diff (ops_of s1) (ops_of lca)) > 0 /\
+             Seq.length (diff (ops_of s2) (ops_of lca)) > 0 /\
+             is_prefix (ops_of lca) (ops_of (inverse_st s1)) /\
+             is_prefix (ops_of lca) (ops_of (inverse_st s2)) /\
              concrete_merge_pre (v_of lca) (v_of s1) (v_of s2) /\
              concrete_merge_pre (v_of lca) (v_of (inverse_st s1)) (v_of (inverse_st s2)) /\
              interleaving_predicate l' lca (inverse_st s1) (inverse_st s2))
@@ -107,3 +125,18 @@ let linearizable_s1s2_gt0 (lca s1 s2:st) (l':log)
   lem_foldl (v_of (linearized_merge (v_of lca) l')) (resolve_conflict (last (ops_of s1)) (last (ops_of s2)));
   Seq.lemma_append_count l' (resolve_conflict (last (ops_of s1)) (last (ops_of s2)))
 
+
+
+
+
+
+  (*)let resolve_conflict_len (x y:log_entry)
+   : Lemma (Seq.length (resolve_conflict x y) = 2)
+   = ()
+
+   let resolve_conflict_mem (x y:log_entry)
+   : Lemma (resolve_conflict_len x y;
+                                 let s = resolve_conflict x y in
+                                 (Seq.length s == 1 ==> is_x_or_y s x y) /\
+                                 (Seq.length s == 2 ==> is_x_and_y s x y))
+   = ()*)
